src/FrameStack/Vulnerabilities/Reachability.v
@@ -1,0 +1,263 @@
+(**
+ * In this file we aim to implement reachability logic proof system as defined
+ * in https://fsl.cs.illinois.edu/publications/rosu-stefanescu-ciobaca-moore-2013-lics.pdf
+ * The ultimate goal is to come up with an implementation that would allow us
+ * to reason about label trace in iterative / loop constructs.
+ *)
+
+From CoreErlang.FrameStack Require Export SubstSemanticsLabeledLemmas.
+From stdpp Require Import list.
+Import ListNotations.
+
+Definition flush_hyps (C: list Prop) (g: Prop) : Prop :=
+  foldr (fun h acc => h -> acc) g C.
+
+Lemma reach_trans (C: list Prop) :
+  forall (fs fs' fs'': FrameStack) (e e' e'': Redex) (l l': list SideEffect),
+  (* all of Props in C are result of reach_circu *) 
+  ⟨ fs, e ⟩ -[ l ]->* ⟨ fs', e' ⟩ (* reaches C fs e l fs' e' *) ->
+  flush_hyps C (⟨ fs', e' ⟩ -[ l' ]->* ⟨ fs'', e'' ⟩) ->
+  ⟨ fs, e ⟩ -[ l ++ l' ]->* ⟨ fs'', e'' ⟩.
+Proof.
+  intros. generalize dependent C.
+  induction C; simpl; intro.
+  - apply (transitive_any_eval H H0).
+  - Abort.
+
+reaches C fs e l fs' e' -> ⟨ fs, e ⟩ -[ l ]->* ⟨ fs', e' ⟩
+
+(* Definition reaches (C: list Prop) :
+  FrameStack -> Redex -> list SideEffect -> FrameStack -> Redex -> Prop
+:=
+  fun fs r l fs' r' =>
+    reach_refl C fs r l fs' r' \/
+
+Lemma reach_trans (C: list Prop) :=
+  forall fs r l fs' r' l' fs'' r'':
+  reaches *)
+
+Inductive PSD (C: list Prop):
+  FrameStack -> Redex -> list SideEffect -> FrameStack -> Redex -> Prop :=
+(* Proof system rules *)
+
+(*
+  No Axiom rule. Instead we would use rules from "step" or use hypotheses
+  which were flushed into the context using "flush_hyps".
+*)
+
+(* Reflexivity *)
+| psd_reflx fs r:
+  length C = 0 -> PSD C fs r [] fs r
+
+(* Transitivity *)
+| psd_trans fs r l fs' r' l' fs'' r'':
+  PSD C fs r l fs' r' ->
+  flush_hyps C (PSD [] fs' r' l' fs'' r'') ->
+  PSD C fs r (l ++ l') fs'' r''.
+
+(**
+ * Below is the original content of proof_system.v. I will try to adapt it to our 
+ * semantics (in other words, remove the generalisation)
+ *)
+
+Section domain.
+Variable cfg : Set.
+
+(* Because we are showing soundness, it's a stronger result if we don't put any
+   restrictions on the syntax or domains of matching logic patterns,
+   so we instead allow an arbitrary satisfaction relation.
+ *)
+Definition formula env : Type := env -> cfg -> Prop. (* pattern *)
+Definition stateless env : Type := env -> Prop.      (* boolean claims *)
+
+(* Rather than explicitly tagging rules as one-path or all-path,
+   observe that none of the rules mix quantifiers, so we'll just
+   state the proof system without saying whether it's one-path or
+   all-path, and prove that soundness for both interpretations.
+ *)
+Definition system := forall env,
+  formula env -> formula env -> Prop.
+
+Definition my_system :=
+  FrameStack -> Redex -> list SideEffect -> FrameStack -> Redex -> Prop.
+
+Definition in_opt_system (S : option system) env (phi phi' : formula env) : Prop :=
+  match S with
+    | None => False
+    | Some sys => sys env phi phi'
+  end.
+
+Definition cons_system env (phi phi' : formula env) (S : system) : system :=
+  fun env0 X X0 =>
+    S env0 X X0 \/
+    {H : env = env0 | phi = eq_rect_r _ X H /\ phi' = eq_rect_r _ X0 H}.
+
+Definition cons_opt_system env (phi phi' : formula env) (S : option system) : option system :=
+  Some (cons_system env phi phi' (in_opt_system S)).
+
+Definition system_empty (S : option system) : Prop :=
+  match S with
+    | Some _ => False
+    | None => True
+  end.
+
+Definition union_system (C : option system) (S : system) : system :=
+  match C with
+    | None => S
+    | Some S1 =>
+      fun env0 X X0 => S1 env0 X X0 \/ S env0 X X0
+  end.
+
+Section FixTransition.
+Variable (S : cfg -> cfg -> Prop).
+
+Search fst.
+
+(* The proof system defined for soundness.
+   Because we are only interested in soundness here, including additional
+   rules is a stronger result (such as allowing logical framing at any
+   point rather than just combined with axiom, including substitution
+   as an explicit rule, or including step even during the
+   one-path soundness proof)
+ *)
+Inductive IS (C : option system) (A : system) : forall env,
+  formula env -> formula env -> Prop :=
+  (* This step is written in terms of a transtion relation, rather
+     than a system given as a set of rules.
+     Equavalence to the version in the paper is shown
+     later in this file. *)
+  | is_step : forall env (phi phi' : formula env),
+                (forall e c, phi e c ->
+                             (exists c2, S c c2) /\
+                             (forall c2, S c c2 -> phi' e c2)) ->
+                 IS C A env phi phi' (* won't be needed since fss is determenistic *)
+  (* if we can make a step / transition *)
+  | is_axiom : forall env phi phi',
+                 A env phi phi' -> IS C A env phi phi'
+  (* if there is a step fs, e -[l]->* fs' e' *)
+  | is_refl : forall env phi, system_empty C -> IS C A env phi phi
+  | is_trans : forall env phi phi' phi'',
+       IS C A env phi phi' ->
+       IS None (union_system C A) env phi' phi'' ->
+       IS C A env phi phi''
+  | is_conseq : forall env
+       (phi1 phi1' phi2 phi2' : formula env),
+       (forall e g, phi1 e g -> phi1' e g) ->
+       (forall e g, phi2 e g -> phi2' e g) ->
+       IS C A env phi1' phi2 ->
+       IS C A env phi1 phi2'
+  | is_case : forall env phi phi1 phi',
+       IS C A env phi  phi' ->
+       IS C A env phi1 phi' ->
+       IS C A env (fun e g => phi e g \/ phi1 e g) phi'
+(* Abstraction with frehsness made manifest by giving phi a biggern env. *)
+  | is_abstr : forall env denx
+       (phi : formula (env * denx)) (phi' : formula env),
+       IS C A (env * denx) phi (fun rho_and_x g => phi' (fst rho_and_x) g) ->
+       IS C A env (fun rho g => exists x, phi (rho , x) g) phi'
+(* Abstraction done by replacing the value in the environment,
+   with the operation (repx) of replacing that value in the environment left abstract,
+   and freeness of phi' taken as an assumption. *)
+  | is_abstr' : forall env denx repx
+       (phi phi' : formula env),
+       (forall rho (x : denx) gamma, phi' rho gamma <-> phi' (repx x rho) gamma) ->
+       IS C A env phi phi' ->
+       IS C A env (fun rho g => exists x, phi (repx x rho) g) phi'
+  | is_circ : forall env phi phi',
+       IS (cons_opt_system env phi phi' C) A env phi phi' ->
+       IS C A env phi phi'
+  | is_subst : forall env env' f phi phi',
+       IS C A env' phi phi' ->
+       IS C A env (fun e g => phi (f e) g) (fun e g => phi' (f e) g)
+  | is_lf : forall env phi phi' psi,
+       IS C A env phi phi' ->
+       IS C A env (fun e g => phi e g  /\ psi e)
+                  (fun e g => phi' e g /\ psi e).
+
+(* Now some lemmas checking adequacy of definitions that
+   won't be needed outside this file
+ *)
+
+(* For soundness, the weakly-well-defined condition is used mostly
+   just to be sure that the transition system induced by a set of
+   rules actually makes it's own rules semantically valid.
+   Check that here. *)
+(* A transition relation where each rule in the system
+   induces an immediate step *)
+Definition relation_of_system (S : system) : cfg -> cfg -> Prop :=
+  fun gamma gamma' =>
+    exists env, exists (rho : env), exists phi, exists phi',
+       (S env phi phi') /\ phi rho gamma /\ phi' rho gamma'.
+(* A system consisting of rules all of whose instances
+   hold in exactly one step along some path *)
+Definition system_of_relation (R : cfg -> cfg -> Prop) : system :=
+  fun env phi phi' =>
+    forall (rho : env) gamma gamma',
+      phi rho gamma -> phi' rho gamma' -> R gamma gamma'.
+(* A weakly well-defined rule *)
+Definition weakly_well_defined (env : Set) phi phi' : Prop :=
+  forall (gamma : cfg) (rho : env), phi rho gamma -> exists (gamma' : cfg), phi' rho gamma'.
+(* Show that the if a rule is weakly-well-defined, then included in the
+   system of the transition relation of any system including that rule *)
+Lemma weakly_well_defined_rule_valid :
+  forall (S : system) (env : Set) (phi phi' : formula env),
+    S env phi phi' -> weakly_well_defined env phi phi' ->
+    (system_of_relation (relation_of_system S) env phi phi').
+unfold system_of_relation, relation_of_system; eauto 40.
+Qed.
+
+Section StepGood.
+Variable (Ssys : system).
+Hypothesis (Ssys_welldef :
+              forall env phi phi' e c1,
+                (Ssys env phi phi' /\ phi e c1) ->
+                exists c2, phi' e c2).
+Hypothesis (Ssys_good :
+              forall c1 c2, S c1 c2 <->
+                            exists env phi phi' e,
+              (Ssys env phi phi' /\ phi e c1 /\ phi' e c2)).
+
+(* Check that the step rule is faithful compared to the
+   paper proof as long as S is generated from
+   a set of sell-defined reachability rules *)
+
+Lemma s_prog :
+  forall c,
+    (exists c2, S c c2)
+      <-> (exists env phi phi' e,
+            Ssys env phi phi' /\ phi e c).
+split. firstorder eauto.
+intros.
+destruct H as (env & phi & phi' & e & H).
+specialize (@Ssys_welldef env phi phi' e c H).
+destruct Ssys_welldef.
+exists x.
+apply Ssys_good.
+firstorder eauto.
+Qed.
+
+Lemma s_succs :
+  forall env1 (e : env1) c (phi_g : formula env1),
+    ((forall c2, S c c2 -> phi_g e c2)
+      <->
+     (forall env phi phi',
+       Ssys env phi phi' ->
+       forall e2, phi e2 c ->
+                  forall c2, phi' e2 c2 -> phi_g e c2)).
+Proof.
+intros.
+split.
+intros.
+apply H.
+apply Ssys_good.
+firstorder eauto.
+
+intros.
+apply Ssys_good in H0.
+destruct H0 as (env & phi & phi' & e2 & Hssys & Hphi & Hphi').
+apply (H env phi phi' Hssys e2 Hphi c2 Hphi').
+Qed.
+End StepGood.
+End FixTransition.
+
+End domain.
